ClassicalLogic.v
@@ -1,0 +1,51 @@
+Require Import List.
+Import ListNotations.
+
+Require Import Bool.
+
+Parameter V : Type.
+Parameter dec : V -> V -> bool.
+Parameter dec_spec :
+  forall x y : V, reflect (x = y) (dec x y).
+
+Require Import Arith.
+
+Notation "x =? y" := (dec x y) (at level 70).
+
+Inductive Formula : Type :=
+    | Var : V -> Formula
+    | FFalse : Formula
+    | FTrue : Formula
+    | Not : Formula -> Formula
+    | Impl : Formula -> Formula -> Formula
+    | Or : Formula -> Formula -> Formula
+    | And : Formula -> Formula -> Formula.
+
+Definition Iff (P Q : Formula) : Formula :=
+  And (Impl P Q) (Impl Q P).
+
+Definition Valuation : Type := V -> bool.
+
+Fixpoint value (f : Valuation) (F : Formula) : bool :=
+match F with
+    | Var x => f x
+    | FFalse => false
+    | FTrue => true
+    | Not F' => negb (value f F')
+    | Impl F1 F2 => orb (negb (value f F1)) (value f F2)
+    | Or F1 F2 => orb (value f F1) (value f F2)
+    | And F1 F2 => andb (value f F1) (value f F2)
+end.
+
+Definition valid (v : Valuation) (F : Formula) : Prop :=
+  value v F = true.
+
+Definition tautology (F : Formula) : Prop :=
+  forall v : Valuation, valid v F.
+
+Lemma LEM_tautology :
+  forall P : Formula, tautology (Or P (Not P)).
+Proof.
+  unfold tautology, valid, Valuation; cbn; intros.
+  destruct (value v P); cbn; reflexivity.
+Qed.
