IntuitionisticLogic.v
@@ -1,0 +1,114 @@
+Require Import List.
+Import ListNotations.
+
+Require Import Bool.
+
+Parameter V : Type.
+Parameter dec : V -> V -> bool.
+Parameter dec_spec :
+  forall x y : V, reflect (x = y) (dec x y).
+
+Require Import Arith.
+
+Notation "x =? y" := (dec x y) (at level 70).
+
+Inductive Formula : Type :=
+    | Var : V -> Formula
+    | FFalse : Formula
+    | Impl : Formula -> Formula -> Formula
+    | Or : Formula -> Formula -> Formula
+    | And : Formula -> Formula -> Formula.
+
+Definition Not (P : Formula) : Formula := Impl P FFalse.
+Definition Iff (P Q : Formula) : Formula :=
+  And (Impl P Q) (Impl Q P).
+Definition FTrue : Formula := Impl FFalse FFalse.
+
+Definition Context : Type := list Formula.
+
+Inductive Proves : Context -> Formula -> Prop :=
+    | Ax :
+        forall (C : Context) (P : Formula),
+          Proves (P :: C) P
+    | FFalseE :
+        forall (C : Context) (P : Formula),
+          Proves C FFalse -> Proves C P
+    | ImplI :
+        forall (C : Context) (P Q : Formula),
+          Proves (P :: C) Q -> Proves C (Impl P Q)
+    | ImplE :
+        forall (C : Context) (P Q : Formula),
+          Proves C (Impl P Q) -> Proves C P -> Proves C Q
+    | AndI :
+        forall (C : Context) (P Q : Formula),
+          Proves C P -> Proves C Q -> Proves C (And P Q)
+    | AndEL :
+        forall (C : Context) (P Q : Formula),
+          Proves C (And P Q) -> Proves C P
+    | AndER :
+        forall (C : Context) (P Q : Formula),
+          Proves C (And P Q) -> Proves C Q
+    | OrIL :
+        forall (C : Context) (P Q : Formula),
+          Proves C P -> Proves C (Or P Q)
+    | OrIR :
+        forall (C : Context) (P Q : Formula),
+          Proves C Q -> Proves C (Or P Q)
+    | OrE :
+        forall (C : Context) (P Q R : Formula),
+          Proves (P :: C) R -> Proves (Q :: C) R -> Proves C (Or P Q) ->
+            Proves C R.
+
+Hint Constructors Proves.
+
+Lemma weakening :
+  forall (C : Context) (F : Formula),
+    Proves C F -> forall R : Formula, Proves (R :: C) F.
+Proof.
+  induction 1; intros; auto.
+    admit.
+    
+Admitted.
+
+Fixpoint subst (F : Formula) (x : V) (P : Formula) : Formula :=
+match F with
+    | Var y => if x =? y then P else Var y
+    | FFalse => FFalse
+    | Impl F1 F2 => Impl (subst F1 x P) (subst F2 x P)
+    | Or F1 F2 => Or (subst F1 x P) (subst F2 x P)
+    | And F1 F2 => And (subst F1 x P) (subst F2 x P)
+end.
+
+Fixpoint csubst (C : Context) (x : V) (P : Formula) : Context :=
+match C with
+    | [] => []
+    | F :: C' => subst F x P :: csubst C' x P
+end.
+
+Lemma Proves_subst :
+  forall (C : Context) (F : Formula),
+    Proves C F -> forall (R : Formula) (x : V),
+      Proves (csubst C x R) (subst F x R).
+Proof.
+  induction 1; cbn; intros; eauto.
+Qed.
+
+Lemma ImplI' :
+  forall (C : Context) (P Q : Formula),
+    (In P C -> Proves C Q) -> Proves C (Impl P Q).
+Proof.
+  intros C P Q H. apply ImplI.
+Abort.
+
+Ltac inv H :=
+  inversion H; subst; clear H; auto.
+
+(* Definitely too hard. *)
+Lemma consistent :
+  forall C : Context,
+    ~ Proves C FFalse.
+Proof.
+  intros C H. remember FFalse as F. revert HeqF.
+  induction H; intro; try inv HeqF; auto.
+Abort.
+
